cont'd

investigations/bedrock2/LibBase/BitfieldProperties.v
@@ -27,6 +27,7 @@ Require Import Bedrock2Experiments.WhileProperties.
 Require Import Bedrock2Experiments.Word.
 Require Import Bedrock2Experiments.WordProperties.
 Require Import Bedrock2Experiments.LibBase.Bitfield.
+Require Import Bedrock2Experiments.LibBase.LibBaseSemantics.
 
 Require Import coqutil.Map.SortedListString.
 Import Syntax.Coercions List.ListNotations.
@@ -34,47 +35,9 @@ Local Open Scope string_scope.
 Local Open Scope list_scope.
 Local Open Scope Z_scope.
 
-Class parameters :=
-  { word :> Interface.word.word 32;
-    mem :> Interface.map.map word Byte.byte;
-    ext_spec : list
-    (mem * string * list word *
-    (mem * list word)) ->
-    mem ->
-    string ->
-    list word ->
-    (mem -> list word -> Prop) -> Prop
-  }.
-
-Instance semantics_parameters {p : parameters}: Semantics.parameters :=
-{|
-  Semantics.width := 32;
-  Semantics.word := word;
-  Semantics.mem := mem;
-  Semantics.locals := SortedListString.map _;
-  Semantics.env := SortedListString.map _;
-  Semantics.ext_spec := ext_spec;
-|}.
-
-Class ok (p : parameters) :=
-  {  word_ok :> word.ok word;
-    mem_ok :> Interface.map.ok mem;
-    ext_spec_ok :> ext_spec.ok semantics_parameters;
-  }.
-
-Instance semantics_parameters_ok {p : parameters} {ok : ok p}: Semantics.parameters_ok semantics_parameters.
-Proof.
-  split.
-  - cbv. left. reflexivity.
-  - exact word_ok.
-  - exact mem_ok.
-  - exact (SortedListString.ok _).
-  - exact (SortedListString.ok _).
-  - exact ext_spec_ok.
-Qed.
-
 Section Proof.
-  Context {p : parameters} {p_ok : ok p}.
+  Import LibBaseSemantics.
+  Context {p : parameters} {p_ok : parameters_ok p}.
 
   Instance spec_of_bitfield_field32_write : spec_of "b2_bitfield_field32_write" :=
     fun function_env =>
@@ -86,12 +49,6 @@ Section Proof.
   Lemma bitfield_field32_write_correct :
     program_logic_goal_for_function! bitfield_field32_write.
   Proof.
-    repeat straightline.
-    repeat split; try reflexivity.
-    cbv [bitfield0] in *.
-    Search word.or.
-    exists bitfield.
-    repeat split; try reflexivity.
     Admitted.
 
   Instance spec_of_bitfield_field32_read : spec_of "b2_bitfield_field32_read" :=
