investigations/bedrock2/LibBase/AbsMMIOProperties.v
@@ -1,0 +1,54 @@
+Require Import Coq.Strings.String.
+Require Import Coq.Lists.List.
+Require Import Coq.micromega.Lia.
+Require Import Coq.ZArith.ZArith.
+Require Import bedrock2.Array.
+Require Import bedrock2.Map.Separation.
+Require Import bedrock2.Map.SeparationLogic.
+Require Import bedrock2.ProgramLogic.
+Require Import bedrock2.Scalars.
+Require Import bedrock2.Semantics.
+Require Import bedrock2.Syntax.
+Require Import bedrock2.TailRecursion.
+Require Import bedrock2.WeakestPrecondition.
+Require Import bedrock2.WeakestPreconditionProperties.
+Require Import coqutil.Word.Interface.
+Require Import coqutil.Word.Properties.
+Require Import coqutil.Map.Interface.
+Require Import coqutil.Map.Properties.
+Require Import coqutil.Tactics.Tactics.
+Require Import coqutil.Tactics.syntactic_unify.
+Require Import coqutil.Tactics.letexists.
+Require Import coqutil.Z.Lia.
+Require Import Cava.Util.List.
+Require Import Cava.Util.Tactics.
+Require Import Bedrock2Experiments.Tactics.
+Require Import Bedrock2Experiments.WhileProperties.
+Require Import Bedrock2Experiments.Word.
+Require Import Bedrock2Experiments.WordProperties.
+Require Import Bedrock2Experiments.LibBase.AbsMMIO.
+Require Import Bedrock2Experiments.LibBase.LibBaseSemantics.
+Require Import coqutil.Map.SortedListString.
+
+Import Syntax.Coercions List.ListNotations.
+Local Open Scope string_scope.
+Local Open Scope list_scope.
+Local Open Scope Z_scope.
+
+Section Proof.
+  Import LibBaseSemantics.
+  Context {p : parameters} {p_ok : parameters_ok p}.
+
+  Instance spec_of_abs_mmio_read32 : spec_of "abs_mmio_read32" :=
+    fun function_env =>
+      forall (addr : word) (R : mem -> Prop) (m : mem) (t : trace),
+        call function_env abs_mmio_read32 t m [addr]
+        (fun t' m' rets => t = t' /\ m = m').
+
+  Check ( _ : spec_of abs_mmio_read32).
+  Lemma abs_mmio_read32_correct :
+    program_logic_goal_for_function! abs_mmio_read32.
+  Proof.
+  Admitted.
+
+End Proof.
